

# Functional Analysis (MA 8673) Homework 1

Kevin Ho

February 9, 2026

1. Define

$$A = i \frac{d}{dx}$$

on  $L^2[0,1]$ . Define two domains for  $A$  :  $\mathcal{D}_1(A) = AC[0,1]$  and  $\mathcal{D}_2(A) = \{f \in AC[0,1] : f(0) = 0\}$ . Prove that  $A$  is closed on  $\mathcal{D}_1(A)$ . Prove or disprove  $A$  is closed on  $\mathcal{D}_2(A)$

*Proof.* Let  $\{f_n\} \in AC[0,1]$  such that  $f_n \rightarrow f \in L^2[0,1]$  and  $Af_n \rightarrow g \in L^2$ . Note that  $Af_n = if'_n$  and so  $if'_n \rightarrow g = f'_n \rightarrow -ig$ .

For simplicity let  $-ig = h$ . Another thing to note, since we are in a finite space of  $[0,1]$ , by Holder's inequality,  $f'_n \rightarrow h \in L^1[0,1]$ . So now let's observe the integration of the sequence of  $f_n$ . By FTOC we get,

$$\int_0^x f'_n(t)dt = f_n(x) - f_n(0) \tag{1}$$

$$\rightarrow f_n(0) = f_n(x) - \int_0^x f'_n(t)dt$$

Since we know this converges in  $L^1$ , we integrate both sides w.r.t.  $x$  to get

$$\int_0^1 f_n(0)dx = \int_0^1 f_n(x)dx - \int_0^1 \int_0^x f'_n(t)dt dx$$

$$\rightarrow f_n(0) = \int_0^1 f_n(x)dx - \int_0^1 \int_0^x f'_n(t)dt dx$$

Let  $c = \lim_{n \rightarrow \infty} f_n(0)$ . (We know this limit exists because the RHS terms converge).

Now let's go back to (1) to get the relation

$$f_n(x) = f_n(0) + \int_0^x f'_n(t)dt$$

Taking the limit as  $n \rightarrow \infty$ :

$$f(x) = c + \int_0^x h(t) dt$$

This equation tells us two things:

- (a) The function  $f$  is absolutely continuous (since it is an integral of an  $L^1$  function), so  $f \in \mathcal{D}_1(A)$ .
- (b) Differentiating both sides gives  $f'(x) = h(x)$ .

Recall that  $h = -ig$ . Therefore:

$$f' = -ig \implies if' = g \implies Af = g$$

Thus,  $A$  is closed on  $\mathcal{D}_1(A)$ .

So now let's observe  $\{f_n\} \in \mathcal{D}_2(A)$ . Assume all the earlier assumptions as shown for  $\mathcal{D}_1(A)$ . Since  $f_n \in \mathcal{D}_2(A)$ , we have  $f_n(0) = 0$ . By FTOC we have

$$f_n(x) = \int_0^x f'_n(t) dt.$$

Now for any  $x \in [0, 1]$ , we bound the difference by

$$|f_n(x) - \int_0^x h(t) dt| \leq \int_0^x |f'_n(t) - h(t)| dt \leq \|f'_n - h\|_{L^1}$$

Now assume  $f_n \in \mathcal{D}_2(A)$ , so  $f_n(0) = 0$  for all  $n$ . Hence  $c = \lim_{n \rightarrow \infty} f_n(0) = 0$ , and so the function

$$F(x) = c + \int_0^x h(t) dt$$

satisfies  $F(0) = 0$ , i.e.  $F \in \mathcal{D}_2(A)$ . From the estimate above we already have  $f_n \rightarrow F$  in  $L^2$ , hence  $f = F$  a.e. Also  $F' = h = -ig$  a.e., so  $Af = g$ . Therefore  $A$  is closed on  $\mathcal{D}_2(A)$ .

□

2. Let  $A$  and  $B$  be operators defined on a Hilbert space  $\mathcal{H}$ . Show that  $(\alpha A)^* = \bar{\alpha} A^*$  for scalar  $\alpha$ . Moreover show  $A^* + B^* \subseteq (A + B)^*$  where  $\mathcal{D}(A^* + B^*) = \mathcal{D}(A^*) \cap \mathcal{D}(B^*)$ . Show that  $(A + B)^* = A^* + B^*$  only if one of the operators is bounded. Give an example where equality doesn't hold.

*Proof.* Define  $x, y \in \mathcal{H}$  s.t.  $x \in \mathcal{D}(A)$  and  $y \in \mathcal{D}(A^*)$  and  $\alpha$  be a scalar. We can manipulate  $\langle (\alpha A)x, y \rangle$  as follows.

$$\alpha \langle x, A^* y \rangle = \langle x, \bar{\alpha} A^* y \rangle$$

This implies that  $y \in ((\alpha A)^*)$  and so  $(\alpha A)^* y = \bar{\alpha} A^* y$

Now let's show that  $A^* + B^* \subseteq (A + B)^*$ .

$$\begin{aligned} \langle (A + B)x, y \rangle &= \langle Ax, y \rangle + \langle Bx, y \rangle \\ &= \langle x, A^* y \rangle + \langle x, B^* y \rangle \\ &= \langle x, (A + B)^* y \rangle \end{aligned}$$

This holds  $\forall x \in \mathcal{D}(A + B)$ , it follows that  $y \in ((A + B)^*)$  and  $(A + B)^* y = (A^* + B^*)y$ .

Assume  $A$  is bounded. Then  $\mathcal{D}(A) = \mathcal{H}$ , which implies  $\mathcal{D}(A^*) = \mathcal{H}$ . Consequently, the domain of the sum simplifies to  $\mathcal{D}(A + B) = \mathcal{D}(B)$ .

From Part 2, we already know  $A^* + B^* \subseteq (A + B)^*$ . We must now show the reverse inclusion  $(A + B)^* \subseteq A^* + B^*$ .

Let  $y \in \mathcal{D}((A + B)^*)$ . By definition, there exists a vector  $z \in \mathcal{H}$  such that for all  $x \in \mathcal{D}(A + B) = \mathcal{D}(B)$ :

$$\langle (A + B)x, y \rangle = \langle x, z \rangle$$

Using the linearity of the inner product, we expand the left side:

$$\langle Ax, y \rangle + \langle Bx, y \rangle = \langle x, z \rangle$$

Since  $A$  is bounded and defined on all of  $\mathcal{H}$ , we know that  $y \in \mathcal{D}(A^*)$  so  $\langle Ax, y \rangle = \langle x, A^* y \rangle$ . Substituting this into the equation, we get

$$\begin{aligned} \langle x, A^* y \rangle + \langle Bx, y \rangle &= \langle x, z \rangle \\ \langle Bx, y \rangle &= \langle x, z \rangle - \langle x, A^* y \rangle \\ \langle Bx, y \rangle &= \langle x, z - A^* y \rangle \end{aligned}$$

This equation holds for all  $x \in \mathcal{D}(B)$ . By the definition of the adjoint, this implies that  $y \in \mathcal{D}(B^*)$  and  $B^* y = z - A^* y$ .

Since  $y \in \mathcal{D}(B^*)$  and  $y \in \mathcal{D}(A^*)$ , we have  $y \in \mathcal{D}(A^*) \cap \mathcal{D}(B^*) = \mathcal{D}(A^* + B^*)$ .

Thus,  $(A + B)^* \subseteq A^* + B^*$  and so we have  $(A + B)^* = A^* + B^*$ .

**Counter Example:** An example of where the inequality doesn't hold is let  $A = -B$ . Also let  $A$  be an unbounded operator. We have the following to occur of  $A + B = 0$  on  $\mathcal{D}(A)$ , so  $(A + B)^* = 0$  on the entire space  $\mathcal{H}$ . Now observing the adjoint of  $(A + B)^*$ , we get  $A^* + B^* = A^* - A^* = 0$ . This implies that the domain is restricted to  $\mathcal{D}(A^*)$ . This implies that the domain of  $A^* + B^*$  is restricted to  $\mathcal{D}(A^*)$ . However, the domain of

$(A + B)^*$  is the entire space  $\mathcal{H}$ . This mismatch between  $\mathcal{D}(A^* + B^*)$  and  $\mathcal{D}((A + B)^*)$  shows that equality does not hold.

□

3. Let  $A$  and  $B$  be operators defined on a Hilbert space  $\mathcal{H}$  such that  $AB$  is densely defined. Prove that  $(AB)^* \supset B^*A^*$ . Moreover if  $B$  is bounded then show  $(BA)^* = A^*B^*$ .

*Proof.* Let  $y \in \mathcal{D}(A^*)$  and  $A^*y \in \mathcal{D}(B^*)$ . Let  $x \in \mathcal{D}(AB)$  so that we have  $Bx \in \mathcal{D}(A)$ . We then have the following

$$\begin{aligned}\langle (AB)x, y \rangle &= \langle A(Bx), y \rangle = \langle Bx, A^*y \rangle \\ &= \langle x, B^*A^*y \rangle\end{aligned}$$

This shows that  $y \in \mathcal{D}((AB)^*)$  and that  $(AB)^* \supset B^*A^*$ . Now we then want to show the other direction of  $(AB)^* \subset B^*A^*$ .

Let  $y \in (BA)^*$ , then  $\exists z \in \mathcal{H}$  such that

$$\langle BAx, y \rangle = \langle x, z \rangle$$

We can rewrite as follows:

$$\langle Ax, B^*y \rangle = \langle x, z \rangle, \forall x \in \mathcal{D}(A).$$

This means that  $B^*y \in \mathcal{D}(A^*)$  and  $A^*(B^*y) = z = (BA)^*y$ . Leading to the equality of  $(BA)^* = A^*B^*$ .

□

4. An alternative way to define a normal operator (to allow for unboundedness) is the following:  $A$  is called **normal** if  $\|Af\| = \|A^*f\|$  for all  $f \in \mathcal{D}(A) = \mathcal{D}(A^*)$ . Prove that if  $A$  is normal then so is  $A + z$  for all  $z \in \mathbb{C}$

*Proof.* So to satisfy this, we must show that  $\mathcal{D}(A + z) = \mathcal{D}((A + z)^*)$  and  $\|(A + z)f\| = \|(A + z)^*f\|, \forall f \in \mathcal{D}$ .

So first let's show the domain equality.

$$(A + z)^* = A^* + \bar{z}$$

Thus, the domain is given as follows.

$$\mathcal{D}((A + z)^*) = \mathcal{D}(A^* + \bar{z}) = \mathcal{D}(A^*)$$

Since  $A$  is normal,  $\mathcal{D}(A + z) = \mathcal{D}(A) = \mathcal{D}(A^*) = \mathcal{D}((A + z)^*)$

Now we want to show the Norm equality. Let  $f \in \mathcal{D}(A)$ . Let's expand out both sides of the equality

$$\|(A + z)f\| = \|(A + z)^*f\|$$

LHS:

$$\begin{aligned} \|(A + z)f\|^2 &= \langle (A + z)f, (A + z)f \rangle \\ &= \langle Af + zf, Af + zf \rangle \\ &= \langle Af, Af \rangle + \langle Af, zf \rangle + \langle zf, Af \rangle + \langle zf, zf \rangle \\ &= \|Af\|^2 + \bar{z}\langle Af, f \rangle + z\langle Af, f \rangle + |z|^2\|f\|^2 \end{aligned}$$

RHS:

$$\begin{aligned} \|(A + z)^*f\|^2 &= \langle (A + z)^*f, (A + z)^*f \rangle \\ &= \langle A^*f + \bar{z}f, A^*f + \bar{z}f \rangle \\ &= \langle A^*f, A^*f \rangle + \langle A^*f, \bar{z}f \rangle + \langle \bar{z}f, A^*f \rangle + \langle \bar{z}f, \bar{z}f \rangle \\ &= \|A^*f\|^2 + z\langle A^*f, f \rangle + \bar{z}\langle A^*f, f \rangle + |z|^2\|f\|^2 \end{aligned}$$

Note that both sides expand to the same term except the first term of both. Note that  $A$  is normal. With that  $\|Af\|^2 = \|A^*f\|^2$ . Thus  $A + z$  is normal. □

5. Using the above definition, prove that normal operators are always closed.

*Proof.* Let  $\{x_n\}$  be a sequence in  $\mathcal{D}(A)$  such that  $x_n \rightarrow x$  and  $Ax_n \rightarrow y$  in  $\mathcal{H}$ . To prove that  $A$  is closed, we must show that  $x \in \mathcal{D}(A)$  and  $Ax = y$ . Since  $\{Ax_n\}$  is a convergent sequence, it is a Cauchy sequence. By the normality condition  $\|Ah\| = \|A^*h\|$ , we have for any  $n, m$ :

$$\|A^*x_n - A^*x_m\| = \|A^*(x_n - x_m)\| = \|A(x_n - x_m)\| = \|Ax_n - Ax_m\|$$

Since  $\{Ax_n\}$  is Cauchy,  $\|Ax_n - Ax_m\| \rightarrow 0$  as  $n, m \rightarrow \infty$ . Therefore,  $\{A^*x_n\}$  is also a Cauchy sequence in  $\mathcal{H}$  and must converge to some limit  $z$ .

We now have:

$$x_n \rightarrow x \quad \text{and} \quad A^*x_n \rightarrow z$$

Recall that the adjoint operator  $A^*$  is always closed. By the definition of closedness applied to  $A^*$ , this implies that  $x \in \mathcal{D}(A^*)$  and  $A^*x = z$ .

Since  $A$  is normal, we are given that  $\mathcal{D}(A) = \mathcal{D}(A^*)$ . Therefore,  $x \in \mathcal{D}(A)$ .

Finally, we must show that  $Ax = y$ . We apply the norm equality to the vector  $x_n - x$  to get

$$\|Ax_n - Ax\| = \|A^*(x_n - x)\| = \|A^*x_n - A^*x\|.$$

When we take the limit as  $n \rightarrow \infty$ , on the right side, since  $A^*x_n \rightarrow z$  and we found  $A^*x = z$ , the term  $\|A^*x_n - A^*x\| \rightarrow 0$ . Thus the left side  $\|Ax_n - Ax\| \rightarrow 0$ , which implies  $Ax_n \rightarrow Ax$ .

Since we originally assumed  $Ax_n \rightarrow y$ , by the uniqueness of limits, we must have  $Ax = y$ .

Thus,  $x \in \mathcal{D}(A)$  and  $Ax = y$ , proving that  $A$  is closed.  $\square$